Save the newest version

STLC/Argument.v
@@ -26,136 +26,6 @@ From STLC Require Export PatternMatch.
         [M1 M2] = [M1] (fun hole1 => [M2] (fun hole2 => k (hole1 hole2)))
 *)
 
-Print is_recu.
-
-Fixpoint CPS (k : tm) (func_name : string) (func_body : tm) (continuation : tm -> tm) (naming : nat) (fuel : nat) {struct fuel} : tm :=
-match fuel with | 0 => func_body | S fuel' =>
-  match func_body with
-  | var _ =>
-       let result := continuation func_body in
-       match find_func func_name result with
-       | O => app k result
-       | S n1 => result
-       end
-  | abs x1 t1 =>
-       abs x1 (CPS k func_name t1 continuation naming fuel')
-  | app t1 t2 =>
-       if is_recu func_name func_body then
-       let para_name := append "res" (nat2string naming) in
-       let result := continuation (var para_name) in
-       app func_body (abs para_name
-                      match find_func func_name result with
-                      | O => app k result
-                      | S n1 => result
-                      end)
-       else if is_app_F func_name func_body then
-       match t1 with
-       | app func_name t1' =>
-            CPS k func_name t1'
-            (fun res1 : tm => CPS k func_name t2
-            (fun res2 : tm => continuation (app res1 res2)) (naming + (S n1)) fuel') naming fuel'
-       | _ =>
-            CPS k func_name t1
-            (fun res1 : tm => CPS k func_name t2
-            (fun res2 : tm => continuation (app res1 res2)) (naming + (S n1)) fuel') naming fuel'
-       end
-       else match find_func func_name t1, find_func func_name t2 with
-       | O, O =>
-            app k (continuation func_body)
-       | S n1, O =>
-            CPS k func_name t1 (fun res : tm => continuation (app res t2)) naming fuel'
-       | O, S n2 =>
-            CPS k func_name t2 (fun res : tm => continuation (app t1 res)) naming fuel'
-       | S n1, S n2 =>
-            CPS k func_name t1
-            (fun res1 : tm => CPS k func_name t2
-            (fun res2 : tm => continuation (app res1 res2)) (naming + (S n1)) fuel') naming fuel'
-       end
-  
-  | tconst n =>
-       let result := continuation func_body in
-       match find_func func_name result with
-       | O => app k result
-       | S n1 => result
-       end
-  | tplus t1 t2 =>
-       match find_func func_name t1, find_func func_name t2 with
-       | O, O =>
-            app k (continuation func_body)
-       | S n1, O =>
-            CPS k func_name t1 (fun res : tm => continuation (tplus res t2)) naming fuel'
-       | O, S n2 =>
-            CPS k func_name t2 (fun res : tm => continuation (tplus t1 res)) naming fuel'
-       | S n1, S n2 =>
-            CPS k func_name t1
-            (fun res1 : tm => CPS k func_name t2
-            (fun res2 : tm => continuation (tplus res1 res2)) (naming + (S n1)) fuel') naming fuel'
-       end
-  | tminus t1 t2 =>
-       match find_func func_name t1, find_func func_name t2 with
-       | O, O =>
-            app k (continuation func_body)
-       | S n1, O =>
-            CPS k func_name t1 (fun res : tm => continuation (tminus res t2)) naming fuel'
-       | O, S n2 =>
-            CPS k func_name t2 (fun res : tm => continuation (tminus t1 res)) naming fuel'
-       | S n1, S n2 =>
-            CPS k func_name t1
-            (fun res1 : tm => CPS k func_name t2
-            (fun res2 : tm => continuation (tminus res1 res2)) (naming + (S n1)) fuel') naming fuel'
-       end
-  | tmult t1 t2 =>
-       match find_func func_name t1, find_func func_name t2 with
-       | O, O =>
-            app k (continuation func_body)
-       | S n1, O =>
-            CPS k func_name t1 (fun res : tm => continuation (tmult res t2)) naming fuel'
-       | O, S n2 =>
-            CPS k func_name t2 (fun res : tm => continuation (tmult t1 res)) naming fuel'
-       | S n1, S n2 =>
-            CPS k func_name t1
-            (fun res1 : tm => CPS k func_name t2
-            (fun res2 : tm => continuation (tmult res1 res2)) (naming + (S n1)) fuel') naming fuel'
-       end
-  | tif0 t1 t2 t3 =>
-       match find_func func_name t1 with
-       | O => tif0 t1 (CPS k func_name t2 continuation naming fuel') (CPS k func_name t3 continuation naming fuel')
-       | S n1 => CPS k func_name t1 (fun res : tm => continuation (tif0 res t2 t3)) naming fuel'
-       end
-  
-  | tnil =>
-       let result := continuation func_body in
-       match find_func func_name result with
-       | O => app k result
-       | S n1 => result
-       end
-  | tcons t1 t2 =>
-       match find_func func_name t1, find_func func_name t2 with
-       | O, O =>
-            app k (continuation func_body)
-       | S n1, O =>
-            CPS k func_name t1 (fun res : tm => continuation (tcons res t2)) naming fuel'
-       | O, S n2 =>
-            CPS k func_name t2 (fun res : tm => continuation (tcons t1 res)) naming fuel'
-       | S n1, S n2 =>
-            CPS k func_name t1
-            (fun res1 : tm => CPS k func_name t2
-            (fun res2 : tm => continuation (tcons res1 res2)) (naming + (S n1)) fuel') naming fuel'
-       end
-  | tlcase t1 t2 x1 x2 t3 =>
-       match find_func func_name t1 with
-       | O => tlcase t1 (CPS k func_name t2 continuation naming fuel') x1 x2 (CPS k func_name t3 continuation naming fuel')
-       | S n1 => CPS k func_name t1 (fun res : tm => continuation (tlcase res t2 x1 x2 t3)) naming fuel'
-       end
-  
-  | tlet x1 t1 t2 =>
-       tlet x1 (CPS k func_name t1 continuation naming fuel') (CPS k func_name t2 continuation naming fuel')
-  
-  | tfix t1 =>
-       tfix (CPS k func_name t1 continuation naming fuel')
-  end
-end.
-
 Fixpoint depth (func_name : string) (func_body : tm) : nat :=
   match func_body with
   | var _ =>
@@ -242,6 +112,136 @@ Fixpoint depth (func_name : string) (func_body : tm) : nat :=
        1 + depth func_name t1
   end.
 
+Fixpoint CPS (k : tm) (func_name : string) (func_body : tm) (continuation : tm -> tm) (naming : nat) (fuel : nat) {struct fuel} : tm :=
+match fuel with | 0 => func_body | S fuel' =>
+  match func_body with
+  | var _ =>
+       let result := continuation func_body in
+       match find_func func_name result with
+       | O => app k result
+       | S n1 => result
+       end
+  | abs x1 t1 =>
+       abs x1 (CPS k func_name t1 continuation naming fuel')
+  | app t1 t2 =>
+       if is_recu func_name func_body then
+       let para_name := append "res" (nat2string naming) in
+       let result := continuation (var para_name) in
+       app func_body (abs para_name
+                      match find_func func_name result with
+                      | O => app k result
+                      | S n1 => result
+                      end)
+       else if is_app_F func_name func_body
+       then match (find_func func_name t1 - 1), find_func func_name t2 with
+       | O, O =>
+            app k (continuation func_body) (*impossible*)
+       | S n1, O =>
+            CPS k func_name t1 (fun res : tm => continuation (app res t2)) naming fuel'
+       | O, S n2 =>
+            CPS k func_name t2 (fun res : tm => continuation (app t1 res)) naming fuel'
+       | S n1, S n2 =>
+            CPS k func_name t1
+            (fun res1 : tm => CPS k func_name t2
+            (fun res2 : tm => continuation (app res1 res2)) (naming + (S n1)) fuel') naming fuel'
+       end
+       else match find_func func_name t1, find_func func_name t2 with
+       | O, O =>
+            app k (continuation func_body)
+       | S n1, O =>
+            CPS k func_name t1 (fun res : tm => continuation (app res t2)) naming fuel'
+       | O, S n2 =>
+            CPS k func_name t2 (fun res : tm => continuation (app t1 res)) naming fuel'
+       | S n1, S n2 =>
+            CPS k func_name t1
+            (fun res1 : tm => CPS k func_name t2
+            (fun res2 : tm => continuation (app res1 t2)) (naming + (S n1)) fuel') naming fuel'
+       end
+  
+  | tconst n =>
+       let result := continuation func_body in
+       match find_func func_name result with
+       | O => app k result
+       | S n1 => result
+       end
+  | tplus t1 t2 =>
+       match find_func func_name t1, find_func func_name t2 with
+       | O, O =>
+            app k (continuation func_body)
+       | S n1, O =>
+            CPS k func_name t1 (fun res : tm => continuation (tplus res t2)) naming fuel'
+       | O, S n2 =>
+            CPS k func_name t2 (fun res : tm => continuation (tplus t1 res)) naming fuel'
+       | S n1, S n2 =>
+            CPS k func_name t1
+            (fun res1 : tm => CPS k func_name t2
+            (fun res2 : tm => continuation (tplus res1 res2)) (naming + (S n1)) fuel') naming fuel'
+       end
+  | tminus t1 t2 =>
+       match find_func func_name t1, find_func func_name t2 with
+       | O, O =>
+            app k (continuation func_body)
+       | S n1, O =>
+            CPS k func_name t1 (fun res : tm => continuation (tminus res t2)) naming fuel'
+       | O, S n2 =>
+            CPS k func_name t2 (fun res : tm => continuation (tminus t1 res)) naming fuel'
+       | S n1, S n2 =>
+            CPS k func_name t1
+            (fun res1 : tm => CPS k func_name t2
+            (fun res2 : tm => continuation (tminus res1 res2)) (naming + (S n1)) fuel') naming fuel'
+       end
+  | tmult t1 t2 =>
+       match find_func func_name t1, find_func func_name t2 with
+       | O, O =>
+            app k (continuation func_body)
+       | S n1, O =>
+            CPS k func_name t1 (fun res : tm => continuation (tmult res t2)) naming fuel'
+       | O, S n2 =>
+            CPS k func_name t2 (fun res : tm => continuation (tmult t1 res)) naming fuel'
+       | S n1, S n2 =>
+            CPS k func_name t1
+            (fun res1 : tm => CPS k func_name t2
+            (fun res2 : tm => continuation (tmult res1 res2)) (naming + (S n1)) fuel') naming fuel'
+       end
+  | tif0 t1 t2 t3 =>
+       match find_func func_name t1 with
+       | O => tif0 t1 (CPS k func_name t2 continuation naming fuel') (CPS k func_name t3 continuation naming fuel')
+       | S n1 => CPS k func_name t1 (fun res : tm => continuation (tif0 res t2 t3)) naming fuel'
+       end
+  
+  | tnil =>
+       let result := continuation func_body in
+       match find_func func_name result with
+       | O => app k result
+       | S n1 => result
+       end
+  | tcons t1 t2 =>
+       match find_func func_name t1, find_func func_name t2 with
+       | O, O =>
+            app k (continuation func_body)
+       | S n1, O =>
+            CPS k func_name t1 (fun res : tm => continuation (tcons res t2)) naming fuel'
+       | O, S n2 =>
+            CPS k func_name t2 (fun res : tm => continuation (tcons t1 res)) naming fuel'
+       | S n1, S n2 =>
+            CPS k func_name t1
+            (fun res1 : tm => CPS k func_name t2
+            (fun res2 : tm => continuation (tcons res1 res2)) (naming + (S n1)) fuel') naming fuel'
+       end
+  | tlcase t1 t2 x1 x2 t3 =>
+       match find_func func_name t1 with
+       | O => tlcase t1 (CPS k func_name t2 continuation naming fuel') x1 x2 (CPS k func_name t3 continuation naming fuel')
+       | S n1 => CPS k func_name t1 (fun res : tm => continuation (tlcase res t2 x1 x2 t3)) naming fuel'
+       end
+  
+  | tlet x1 t1 t2 =>
+       tlet x1 (CPS k func_name t1 continuation naming fuel') (CPS k func_name t2 continuation naming fuel')
+  
+  | tfix t1 =>
+       tfix (CPS k func_name t1 continuation naming fuel')
+  end
+end.
+
 Definition CPS_conversion (func : tm) : tm :=
   match func with
   | tfix (abs func_name func_body) =>
@@ -249,6 +249,20 @@ Definition CPS_conversion (func : tm) : tm :=
        tfix (abs func_name (CPS k func_name func_paraed_body (fun res : tm => res) 1 (depth func_name func_paraed_body)))
   | _ => func
   end.
+
+Definition stlc_argument_case4 :=
+  tfix (abs F
+    (abs a
+      (abs b
+        (abs c
+          (tif0 b 3
+            (tplus 1 <{ F (F a (b - 1) c - 2) (F (a - 1) (b - 1) c - 1) (F (a - 1) (b - 2) (c - 1) - 3) }>)))))).
+
+Compute (CPS_conversion stlc_argument_case4). 
+
+Compute (CPS (var k) "F"
+<{ F (F a (b - 1) c - 2) (F (a - 1) (b - 1) c - 1) }>
+(fun res : tm => tplus 1 res) 1 999).
 
 Module examples.
 
@@ -384,5 +398,40 @@ Theorem stlc_argument_case3_correct :
   let output := 54 in
   (<{origin_fun input}> -->* output) /\ (<{CPS_fun input idNat}> -->* output).
 Proof. split. solve_CPS. solve_CPS. Qed.
+
+(*
+  F a b c :=
+    match b with
+    | 0 => 3
+    | S _ => 1 + f (f a (b - 1) c - 2) (f (a - 1) (b - 1) c - 1) (f (a - 1) (b - 2) (c - 1) - 3)
+    end.
+  We can transfer it to CPS-style by hand:
+  F a b c k :=
+    match b with
+    | 0 => k 3
+    | S _ => f a (b - 1) c (fun res1 => f (a - 1) (b - 1) c (fun res2 => f (a - 1) (b - 2) (c - 1)
+             (fun res3 => f (res1 - 2) (res2 - 1) (res3 - 3) (fun res4 => k (1 + res4)))))
+    end.
+*)
+
+Definition stlc_argument_case4 :=
+  tfix (abs F
+    (abs a
+      (abs b
+        (abs c
+          (tif0 b 3
+            (tplus 1 <{ F (F a (b - 1) c - 2) (F (a - 1) (b - 1) c - 1) (F (a - 1) (b - 2) (c - 1) - 3) }>)))))).
+
+Compute (CPS_conversion stlc_argument_case4).
+
+Theorem stlc_argument_case3_correct :
+  let origin_fun := stlc_argument_case3 in
+  let CPS_fun := CPS_conversion stlc_argument_case3 in
+  let input := tcons 2 (tcons 3 (tcons 5 tnil)) in
+  let output := 54 in
+  (<{origin_fun input}> -->* output) /\ (<{CPS_fun input idNat}> -->* output).
+Proof. split. solve_CPS. solve_CPS. Qed.
+
+
 
 End examples.
